Some proof for soundness add_0

optimizations.v
@@ -3,16 +3,63 @@ Require Import Nat.
 Require Import Bool.
 Require Import bbv.Word.
 Require Import List.
-Require Import Coq_EVM.lib.evmModel.
 Require Import Coq_EVM.datatypes.
 Import EVM_Def Concrete Abstract.
 Require Import Coq_EVM.interpreter.
 Import Interpreter SFS.
+(*Require Import Coq_EVM.lib.evmModel.*)
 Import ListNotations.
 
 
-
 (* Enrique *)
+
+(*
+Definition lnat := [2;4;6].
+
+Fixpoint all_true (prop: nat -> Prop) (l: list nat)  : Prop :=
+match l with
+| [] => True
+| h::t => (prop h) /\ (all_true prop t) 
+end.
+
+
+Theorem aaa: forall (l: list nat) (prop: nat -> Prop),
+all_true prop l->
+forall (v pos: nat), nth_error l pos = Some v -> prop v.
+Proof.
+induction l as [| h t IH].
+- intros. destruct pos; try (simpl in H0; discriminate).
+- intros. simpl in H.
+  destruct H as [proph propt].
+  destruct pos as [|pos'].
+  + simpl in H0. injection H0 as H0. rewrite <- H0. assumption.
+  + simpl in H0.
+    pose proof (IH prop propt v pos').
+    apply H in H0. assumption.
+Qed.
+
+Definition myeven (n: nat) :=
+Nat.even n = true.
+Check (myeven).
+
+Theorem all_true_lnat: all_true myeven lnat.
+Proof.
+unfold lnat. simpl. intuition; try (unfold myeven; reflexivity).
+Qed.
+
+Theorem bbb: forall (n: nat) (pos: nat), 
+nth_error lnat pos = Some n -> myeven n.
+Proof.
+apply aaa. apply all_true_lnat.
+Qed.
+*)
+
+
+Definition stack_val_has_value (av: asfs_stack_val) (v: EVMWord) : bool :=
+match av with 
+| Val x => weqb x v
+| _ => false
+end.
 
 (* ADD(0,X) --> X *)
 Fixpoint optimize_map_add_zero1 (fresh_var: nat) (map: asfs_map): 
@@ -21,8 +68,12 @@ match map with
 | [] => None
 | (n, val)::t => if n =? fresh_var then
                  match val with
-                 | ASFSOp ADD [Val WZero; arg2] =>
-                     Some ((n, ASFSBasicVal arg2)::t)
+                 | ASFSOp ADD [arg1; arg2] => 
+                     if stack_val_has_value arg1 EVM_Def.WZero then
+                       Some ((n, ASFSBasicVal arg2)::t)
+                     else if stack_val_has_value arg2 WZero then
+                       Some ((n, ASFSBasicVal arg1)::t)
+                     else None
                  | _ => None
                  end
                  else match optimize_map_add_zero1 fresh_var t with 
@@ -30,6 +81,7 @@ match map with
                       | Some map' => Some ((n, val)::map')
                       end
 end.
+
 
 Definition optimize_func_map (f: nat -> asfs_map -> option asfs_map) 
   (fresh_var: nat) (s: asfs) : option asfs :=
@@ -41,21 +93,175 @@ match s with
     end
 end.
 
+
 Definition optimize_add_zero1 (fresh_var: nat) (s: asfs) : option asfs :=
 optimize_func_map optimize_map_add_zero1 fresh_var s.
 
-Definition coherent_opm (ops: opm) : Prop :=
-True.
+
+Definition equiv_map_eval (m1 m2: asfs_map) (ops: opm): Prop :=
+forall (stack: concrete_stack) (n: nat), 
+  eval_asfs2_elem stack (FreshVar n) m1 ops = 
+  eval_asfs2_elem stack (FreshVar n) m2 ops.
 
 
-Theorem optimize_add_zero1_safe: forall (a1 a2: asfs) (fresh_var: nat)
-  (s: concrete_stack) (ops: opm),
-optimize_add_zero1 fresh_var a1 = Some a2 ->
-eval_asfs s a1 ops = eval_asfs s a2 ops.
-Proof. 
+Lemma eq_eval_opt_add_zero: forall (m1 m2: asfs_map) (ops: opm) (n: nat)
+  (stack: concrete_stack) (elem: asfs_stack_val),
+ops ADD = Some (Op true 2 add) ->
+optimize_map_add_zero1 n m1 = Some m2 ->
+eval_asfs2_elem stack elem m1 ops = eval_asfs2_elem stack elem m2 ops.
+Proof.
+induction m1 as [|h t IH].
+- intros. simpl in H0. discriminate.
+- intros. simpl in H0. destruct h as [hn hv] eqn: eq_h.
+  destruct (hn =? n) eqn: eq_hn_n.
+  + destruct (hv) as [basicval|opval] eqn: eq_hv. 
+    * admit.
+    * admit.
+  + destruct (optimize_map_add_zero1 n t) as [map'|]; try discriminate.
+    
 Admitted.
 
 
+Lemma equiv_map_eval_opt_add_zero: forall (ops: opm) (n: nat) 
+  (map map': asfs_map),
+ops ADD = Some (Op true 2 add) ->
+optimize_map_add_zero1 n map = Some map' ->
+equiv_map_eval map map' ops.
+Proof.
+intros ops n map. revert ops n.
+induction map as [|h t IH].
+- intros. simpl in H0. discriminate.
+- intros. simpl in H0.
+  destruct h as [nh vh] eqn: eq_h.
+  destruct (nh =? n) eqn: eq_nh_n.
+  + admit.
+  + destruct (optimize_map_add_zero1 n t); try discriminate.
+    injection H0 as H0. rewrite <- H0.
+    unfold equiv_map_eval. intros.
+  
+ unfold equiv_map_eval. intros.
+Admitted.
+
+
+Lemma eval_value: forall (stack: concrete_stack) (val: EVMWord) (m: asfs_map)
+  (ops: opm),
+eval_asfs2_elem stack (Val val) m ops = Some val.
+Proof.
+intros. destruct m; try (unfold eval_asfs2_elem; reflexivity).
+Qed.
+
+Lemma eval_var: forall (stack: concrete_stack) (var: nat) (m1 m2: asfs_map)
+  (ops: opm),
+eval_asfs2_elem stack (InStackVar var) m1 ops =
+eval_asfs2_elem stack (InStackVar var) m2 ops.
+Proof.
+intros. destruct m1.
+- destruct m2; try reflexivity.
+- destruct m2; try reflexivity.
+Qed.
+
+Lemma eval_elem_equiv_map: forall (stack: concrete_stack) (elem: asfs_stack_val)
+  (m1 m2: asfs_map) (ops: opm),
+equiv_map_eval m1 m2 ops ->
+eval_asfs2_elem stack elem m1 ops = eval_asfs2_elem stack elem m2 ops.
+Proof.
+intros.
+destruct elem as [val|var|fvar] eqn: eq_elem.
+- rewrite -> eval_value. rewrite -> eval_value. reflexivity.
+- apply eval_var.
+- unfold equiv_map_eval in H. 
+  pose proof (H stack fvar). assumption.
+Qed.
+
+Lemma opt_add_zero_same_preservation: forall (fresh_var: nat) (h1 h2 maxid1 maxid2: nat) 
+  (s1 s2: asfs_stack) (m1 m2: asfs_map),
+optimize_add_zero1 fresh_var (ASFSc h1 maxid1 s1 m1) = 
+  Some (ASFSc h2 maxid2 s2 m2) ->
+h1 = h2 /\ maxid1 = maxid2 /\ s1 = s2.
+Proof.
+intros. unfold  optimize_add_zero1 in H. unfold optimize_func_map in H.
+destruct (optimize_map_add_zero1 fresh_var m1); try discriminate.
+injection H. intros H1 H2 H3 H4.
+split; try assumption.
+split; try assumption.
+Qed.
+
+
+Theorem optimize_add_zero1_safe_gen: forall (stk: asfs_stack) (ops: opm) (fresh_var: nat)
+  (m m': asfs_map) (c: concrete_stack),
+ops ADD = Some (Op true 2 add) ->
+optimize_map_add_zero1 fresh_var m = Some m' ->
+eval_asfs2 c stk m ops = eval_asfs2 c stk m' ops.
+Proof.
+induction stk as [| h t IH].
+- reflexivity.
+- intros. 
+  pose proof (equiv_map_eval_opt_add_zero ops fresh_var m m' H H0) as 
+    Hequiv_m_m'.
+  unfold eval_asfs2. unfold apply_f_list_asfs_stack_val.
+  destruct (eval_asfs2_elem c h m ops) as [h_eval|] eqn: eq_evalh.
+  + pose proof (eval_elem_equiv_map c h m m' ops Hequiv_m_m')
+      as eq_eval_h_m_m'.
+    rewrite <- eq_eval_h_m_m'. rewrite -> eq_evalh.
+    rewrite -> eval_asfs2_ho. rewrite -> eval_asfs2_ho.
+    destruct (eval_asfs2 c t m ops) as [t_eval|] eqn: eq_eval_t_m.
+    * pose proof (IH ops fresh_var m m' c H H0) as eq_eval_t_m_m'.
+      rewrite <- eq_eval_t_m_m'. rewrite -> eq_eval_t_m.
+      reflexivity.
+    * pose proof (IH ops fresh_var m m' c H H0) as eq_eval_t_m_m'.
+      rewrite <- eq_eval_t_m_m'. rewrite -> eq_eval_t_m.
+      reflexivity.
+  + pose proof (eval_elem_equiv_map c h m m' ops Hequiv_m_m')
+      as eq_eval_h_m_m'.
+    rewrite <- eq_eval_h_m_m'. rewrite -> eq_evalh.
+    reflexivity.
+Qed.
+
+
+Theorem optimize_add_zero1_safe: forall (a1 a2: asfs) (fresh_var: nat)
+  (c: concrete_stack) (ops: opm),
+ops ADD = Some (Op true 2 add) ->
+optimize_add_zero1 fresh_var a1 = Some a2 ->
+eval_asfs c a1 ops = eval_asfs c a2 ops.
+Proof.
+(* Using optimize_add_zero1_safe_gen *)
+intros a1 a2 fresh_var c ops HADD Hopt.
+destruct a1 as [h1 maxid1 s1 m1] eqn: eq_a1.
+destruct a2 as [h2 maxid2 s2 m2] eqn: eq_a2.
+unfold optimize_add_zero1 in Hopt.
+unfold optimize_func_map in Hopt.
+destruct (optimize_map_add_zero1 fresh_var m1) as [m'|]eqn: eq_opt_map;
+  try discriminate.
+injection Hopt as eqh1_h2 eqmaxid eqs1s2 eqm'.
+rewrite -> eqh1_h2. rewrite -> eqs1s2. rewrite <- eqm'.
+unfold eval_asfs.
+destruct (length c =? h2); try reflexivity.
+apply optimize_add_zero1_safe_gen with (fresh_var:=fresh_var); try assumption.
+Qed.
+
+
+(*
+Definition l_op := [optimize_add_zero1_gen; optimize_add_mul1_gen, ....]
+
+Theorem t: forall e \in l_op, ASFS a, 
+  e a ops => Some a' ->
+  eval_asfs a opmap = eval a' opmap
+  
+Definition opt_scheme (lopt: list optimizations) (a: ASFS) := ...
+
+Theorem t: (l: list optimization)
+l is subset of l_op ->
+opt_scheme l a = Some a' ->
+eval a opmap = eval a' opmap.
+
+Definition checker (p1 p2: prog) =
+let asfs1 := symb_exec p1 opmap in
+let asfs2 := symb_exec p2 opmap in
+let opt_asfs1 := opt_scheme ([opt1; opt2;....]) a in
+eq_asfs opt_asfs1  asfs2 opmap.
+
+Proof obligations: [opt1; opt2;....] is a sublist of l:op
+*)
 
 
 (* Joseba *)
